Proved trivial determinism claim for Clight, and corrected boundedness guarantee of memory

concurrency/Clight_bounds.v
@@ -1,17 +1,7 @@
 Require Import compcert.lib.Axioms.
 Require Import compcert.lib.Maps.
 
-Require Import concurrency.sepcomp. Import SepComp.
-
-Require Import concurrency.pos.
-Require Import concurrency.scheduler.
-Require Import concurrency.TheSchedule.
-Require Import concurrency.konig.
-Require Import concurrency.addressFiniteMap. (*The finite maps*)
-Require Import concurrency.pos.
-Require Import concurrency.lksize.
-Require Import concurrency.permjoin_def.
-Require Import Coq.Program.Program.
+Require Import concurrency.sepcomp. 
 From mathcomp.ssreflect Require Import ssreflect ssrbool ssrnat ssrfun eqtype seq fintype finfun.
 Set Implicit Arguments.
 
@@ -19,30 +9,90 @@ Set Implicit Arguments.
 Require Import Coq.ZArith.ZArith.
 
 Require Import concurrency.permissions.
-Require Import concurrency.threadPool.
- 
 Require Import compcert.common.Memory. (*for Mem.perm_order'' *)
 Require Import concurrency.bounded_maps.
 
-
-(*Semantics*)
+Require Import sepcomp.semantics_lemmas.
+Require Import Coqlib.
 Require Import veric.Clight_new.
 Require Import veric.Clightnew_coop.
-Require Import sepcomp.event_semantics.
-Require Import veric.Clight_sim.
-Require Import concurrency.ClightSemantincsForMachines.
-
 
 Lemma CLight_Deterministic: forall ge c m c1 m1 c2 m2,
     veric.Clight_new.cl_step ge c m c2 m2 ->
     veric.Clight_new.cl_step ge c m c1 m1 ->
     c1 = c2 /\ m1 = m2.
-                
-Admitted.
+Proof. intros. 
+specialize (cl_corestep_fun _ _ _ _ _ _ _ H H0); intros X; inversion X; subst. split; trivial.
+Qed.
 
-Lemma CLight_step_mem_bound: forall ge c m c' m',
-    veric.Clight_new.cl_step ge c m c' m' ->
-    bounded_maps.bounded_map (snd (getMaxPerm m)) ->
-    bounded_maps.bounded_map (snd (getMaxPerm m')).
-                
-Admitted.
+Definition bnd_from_init m := bounded_maps.bounded_map (snd (getMaxPerm m)) /\ (Mem.mem_access m).1 = fun z k => None.
+                              
+Lemma preserve_bnd: memstep_preserve (fun m m' => bnd_from_init m -> bnd_from_init m'). 
+Proof. econstructor; intros; eauto.
+induction H; intros.
+{ destruct H0; split.
+    unfold getMaxPerm in *. erewrite Mem.storebytes_access; eauto.
+    erewrite Mem.storebytes_access; eauto. }
+{ Transparent Mem.alloc. unfold Mem.alloc in H. Opaque Mem.alloc.
+  inversion H; clear H; subst. 
+  destruct H0; split; simpl in *; trivial.
+  red; intros. red in H.
+    rewrite (PTree.gmap1 (fun f : Z -> perm_kind -> option permission => f^~ Max)
+               p (PTree.set (Mem.nextblock m)
+          (fun (ofs : Z) (_ : perm_kind) => if zle lo ofs && zlt ofs hi then Some Freeable else None)
+          (Mem.mem_access m).2)) in H1.
+    unfold option_map in H1.
+    rewrite PTree.gsspec in H1.
+    destruct (peq p (Mem.nextblock m)); subst. 
+    { inversion H1; clear H1; subst. clear H0 H. red.
+      exists hi, lo; split; intros.
+      { destruct (zle lo p); destruct (zlt p hi); simpl; trivial; omega. }
+      { destruct (zle lo p); destruct (zlt p hi); simpl; trivial; omega. } }
+    { apply (H p); clear H0. rewrite PTree.gmap1. apply H1. } }
+{ generalize dependent m'. generalize dependent m. induction l; intros.
+  { inversion H; clear H; subst. trivial. }
+  { destruct a as [[b lo] hi]. simpl in H. remember (Mem.free m b lo hi) as q; symmetry in Heqq. 
+    destruct q; try discriminate. apply (IHl m0); trivial. clear H IHl m'.
+    rename m0 into m'.
+    Transparent Mem.free. unfold Mem.free in Heqq. Opaque Mem.free.
+    destruct (Mem.range_perm_dec m b lo hi Cur Freeable); try discriminate. 
+    inversion Heqq; clear Heqq; subst.
+    destruct H0 as [? INI]; split. 
+    intros p f F.  simpl.
+      destruct (peq p b); subst.
+      { simpl in F. rewrite PTree.gmap1 in F. unfold option_map in F. rewrite PTree.gss in F. inversion F; clear F; subst.
+        specialize (H b).
+        remember (((getMaxPerm m).2) ! b) as g. destruct g; symmetry in Heqg.
+        { assert (Some o = Some o) by trivial. specialize (H _ H0); clear H0. rename o into g.
+          destruct H as [HI [LO [HHi HLo]]]. unfold getMaxPerm in Heqg. unfold PMap.get. simpl in *.
+          rewrite PTree.gmap1 in Heqg. unfold option_map in Heqg. rewrite INI.
+          destruct (((Mem.mem_access m).2) ! b); try discriminate. inversion Heqg; clear Heqg; subst.
+          exists  HI, LO; split; intros.
+          { destruct (zle lo p); destruct (zlt p hi); simpl; trivial; eauto. } 
+          { destruct (zle lo p); destruct (zlt p hi); simpl; trivial; eauto. } }
+        { clear H. unfold getMaxPerm in Heqg.
+               destruct (zlt lo hi).
+               { assert (A: lo <= lo < hi) by omega. specialize (r _ A).
+                 apply Mem.perm_max in r. unfold Mem.perm, PMap.get in r. 
+                 rewrite PTree.gmap1 in Heqg. unfold option_map in Heqg.
+                 remember (((Mem.mem_access m).2) ! b) as q. destruct q; simpl in *. discriminate.
+                 rewrite INI in r. inversion r. }
+        { simpl in Heqg. rewrite PTree.gmap1 in Heqg. unfold option_map in Heqg. unfold PMap.get.
+          remember (((Mem.mem_access m).2) ! b) as w. destruct w; try discriminate. clear Heqg.
+          rewrite INI.
+          exists lo, lo; split; intros.
+          { destruct (zle lo p); destruct (zlt p hi); simpl; trivial. }
+          { destruct (zle lo p); destruct (zlt p hi); simpl; trivial. } } } }
+      { apply (H p). unfold getMaxPerm in *; simpl in *.
+        rewrite PTree.gmap1 in F. rewrite PTree.gmap1. unfold option_map in *.
+        rewrite PTree.gso in F; trivial. }
+    simpl; trivial. } }
+eauto.
+Qed.
+
+Lemma CLight_step_mem_bound ge c m c' m':
+    veric.Clight_new.cl_step ge c m c' m' -> bnd_from_init m -> bnd_from_init m'.
+Proof.
+ intros. 
+ apply (memsem_preserves CLN_memsem _ preserve_bnd _ _ _ _ _ H H0).
+Qed. 
